Carry to micro as well

CpcMicro/Spec.lean
@@ -65,7 +65,7 @@ def __eo_to_smt : Term -> SmtTerm
   | (Term.Rational r) => (SmtTerm.Rational r)
   | (Term.String s) => (SmtTerm.String s)
   | (Term.Binary w n) => (SmtTerm.Binary w n)
-  | (Term.Var s T) => (SmtTerm.Var s (__eo_to_smt_type T))
+  | (Term.Var (Term.String s) T) => (SmtTerm.Var s (__eo_to_smt_type T))
   | (Term.UConst i T) => (SmtTerm.UConst (smt_lit_uconst_id i) (__eo_to_smt_type T))
   | (Term.Apply Term.not x1) => (SmtTerm.Apply SmtTerm.not (__eo_to_smt x1))
   | (Term.Apply (Term.Apply Term.or x1) x2) => (SmtTerm.Apply (SmtTerm.Apply SmtTerm.or (__eo_to_smt x1)) (__eo_to_smt x2))
